ConnectionTable: recalling cookies works

src/tls/experiments/ConnectionTable/ConnectionTable.fst
@@ -9,13 +9,14 @@ open FStar.Ghost
 
 module T = FStar.Monotonic.DependentMap
 module DM = FStar.DependentMap
+module B = LowStar.Buffer
+module AEAD = Crypto.AEAD
+module AE = Crypto.AE
+module EE = EverCrypt.Error
 
 open ConnectionTable_Aux
 
-// For the sake of testing extraction
-[@"opaque_to_smt"]
-let model = false
-
+// References to connections live in pairwise disjoint regions
 let minv (m:partial_dependent_map maybe_id connection_ref) =
   forall id1 id2.{:pattern (Some? (DM.sel m id1)); (Some? (DM.sel m id2))}
     (id1 <> id2 /\ Some? (DM.sel m id1) /\ Some? (DM.sel m id2)) ==>
@@ -24,19 +25,18 @@ let minv (m:partial_dependent_map maybe_id connection_ref) =
 let empty = T.empty
 
 val connection_inv:
-    m:T.imap maybe_id connection_ref minv
-  -> c:connection
+    T.imap maybe_id connection_ref minv
+  -> connection
   -> Type0
 let connection_inv m c =
   if model then
     match c with
-    | Sent_ServerHello r ch id1 | Complete r ch id1 ->
+    | Sent_ServerHello ch id1 | Complete ch id1 ->
       if has_cookie ch then
         match T.sel m id1 with
         | Some c' ->
           token_p c' (fun h0 ->
             Sent_HRR? (sel h0 c') /\
-            nonce_of (sel h0 c') == r /\
             ch_of_cookie ch == Sent_HRR?.ch (sel h0 c'))
         | _ -> False
       else True
@@ -57,6 +57,45 @@ let alloc _ =
   if model then
     T.alloc () <: _connection_table
   else ()
+
+#set-options "--max_fuel 0 --max_ifuel 0 --z3rlimit 30"
+
+let table : connection_table = 
+  recall_region rgn;
+  witness_region rgn;
+  alloc ()
+
+val key : b:B.lbuffer UInt8.t 16{B.recallable b}
+let key = 
+  B.gcmalloc_of_list
+    cookie_rgn
+    [ 0x00uy; 0x01uy; 0x02uy; 0x03uy;
+      0x04uy; 0x05uy; 0x06uy; 0x07uy;
+      0x08uy; 0x09uy; 0x0Auy; 0x0Buy;
+      0x0Cuy; 0x0Duy; 0x0Euy; 0x0Fuy ]
+
+let phi s = 
+  Seq.length s >= 32 /\
+  (if model then
+    let random = Seq.slice s 0 32 in
+    let id = id_of_random random in
+    let t:_connection_table = table in
+    token_p t (fun h -> 
+      T.defined t id h /\
+      (let c = T.value_of t id h in
+      token_p c (fun h' -> 
+        Sent_HRR? (sel h' c) /\
+        CH1 random == Sent_HRR?.ch (sel h' c))))
+   else True)
+
+let cookie_key : option (k:AE.state alg phi{model ==> AE.safe k}) =
+  B.recall key;
+  if model then
+    Some (AE.create cookie_rgn alg key phi)
+  else
+    AE.coerce cookie_rgn alg key phi
+
+#set-options "--max_fuel 0 --max_ifuel 1 --z3rlimit 10"
 
 let create t id cfg =
   if model then
@@ -109,9 +148,10 @@ let token_functoriality #a #rel r p q =
 let receive_client_hello1 t id c ch =
   let h0 = get () in
   if ch_compatible ch (Init?.cfg !c) then
-    c := Sent_ServerHello (ch_random ch) ch (if model then 0ul else ())
+    let id0 : maybe_id = if model then 0uy else () in
+    c := Sent_ServerHello ch id0
   else
-    c := Sent_HRR (ch_random ch) ch;
+    c := Sent_HRR ch;
   if model then
     let h1 = get () in
     let t:_connection_table = t in
@@ -119,33 +159,81 @@ let receive_client_hello1 t id c ch =
       forall (id:connection_id).{:pattern (T.defined t id h1)}
         T.defined t id h1 ==> T.defined t id h0)
 
-//[@"opaque_to_smt"]
-let validate_cookie t ch2 =
-  if model then
+assume val random_of_buffer: b:B.buffer UInt8.t -> ST random
+  (requires  fun h -> B.live h b /\ B.length b >= 32)
+  (ensures   fun h0 r h1 -> h0 == h1 /\ r == Seq.slice (B.as_seq h0 b) 0 32)
+
+val validate_cookie':
+    ck:cookie
+  -> Stack (option (maybe_id & random))
+  (requires fun h0 ->
+    Some? cookie_key /\
+    AE.invariant h0 (Some?.v cookie_key) /\ 
+    B.live h0 ck /\
+    (model ==> inv table h0))
+  (ensures  fun h0 o h1 ->
+    B.modifies (AE.footprint (Some?.v cookie_key)) h0 h1 /\
+    AE.invariant h1 (Some?.v cookie_key) /\ 
+    (match o with
+    | None -> True
+    | Some (id, random) ->
+      if model then
+        let t:_connection_table = table in
+        id == id_of_random random /\
+        T.defined t id h0 /\
+        (let c = T.value_of t id h0 in
+           token_p c (fun h ->
+             Sent_HRR? (sel h c) /\
+             CH1 random == Sent_HRR?.ch (sel h c)))
+      else True))
+
+let validate_cookie' ck =
+  let h0 = get () in
+  match cookie_key with
+  | None -> None
+  | Some cookie_key ->
     begin
-    let h0 = get () in
-    // For the sake of testing extraction, return always id1 = 0ul
-    assume (
-      let t:_connection_table = t in
-      let id1 = 0ul in
-      T.defined t id1 h0 /\
-      (let c' = T.value_of t id1 h0 in
-        token_p c' (fun h0 ->
-          Sent_HRR? (sel h0 c') /\
-          nonce_of (sel h0 c') == ch_random ch2 /\
-          ch_of_cookie ch2 == Sent_HRR?.ch (sel h0 c'))));
-    Some 0ul
+    push_frame();
+    let plain = B.alloca 0uy 64ul in
+    let h1 = get () in
+    AE.frame_invariant h0 cookie_key B.loc_none h1;
+    assume (B.loc_includes (B.loc_region_only true cookie_rgn) (AE.footprint cookie_key));
+    assume (B.loc_disjoint (AE.footprint cookie_key) (B.loc_buffer ck));
+    let res : option (maybe_id & random) =
+      match AE.decrypt cookie_key ck 92ul plain with
+      | EE.AuthenticationFailure -> None
+      | EE.Success ->
+        let random = random_of_buffer plain in
+        let id = id_of_random random in
+        if model then
+          let h2 = get () in
+          assert (phi (B.as_seq h2 plain));
+          let t:_connection_table = table in
+          recall_p t (fun h -> 
+            T.defined t id h /\
+            (let c = T.value_of t id h in
+             token_p c (fun h' -> 
+             Sent_HRR? (sel h' c) /\
+             CH1 random == Sent_HRR?.ch (sel h' c))));
+          Some (id, random)
+        else Some ((), random)
+    in
+    pop_frame();
+    let h1 = get () in
+    assume (B.modifies B.loc_none h0 h1);
+    AE.frame_invariant h0 cookie_key B.loc_none h1;
+    res
     end
-  else Some ()
+
 
 let receive_client_hello2 t id c ch2 =
   let h0 = get () in
   match validate_cookie t ch2 with
   | None -> false
-  | Some id1 -> 
+  | Some id0 -> 
     if ch_compatible ch2 (Init?.cfg !c) then
       begin
-      c := Sent_ServerHello (ch_random ch2) ch2 id1;
+      c := Sent_ServerHello ch2 id0;
       let h1 = get () in
       assert (
         if model then
@@ -161,8 +249,7 @@ let receive_client_hello2 t id c ch2 =
 let receive_client_finished t id c =
   let c0 = !c in
   let h0 = get() in
-  c := Complete (Sent_ServerHello?.random c0)
-               (Sent_ServerHello?.ch c0)
+  c := Complete (Sent_ServerHello?.ch c0)
                (Sent_ServerHello?.id1 c0);
   let h1 = get () in
   assert (
