src/tls/experiments/ConnectionTable/Test.fst
@@ -5,52 +5,43 @@ open ConnectionTable
 
 open FStar.HyperStack.ST
 
-#set-options "--z3rlimit 100"// --max_fuel 0 --max_ifuel 0"
+#set-options "--z3rlimit 100 --max_fuel 0 --max_ifuel 0"
 
 (*
    This tests the server side of a full handshake with mismatched parameters:
 
    1. Allocate an empty connection table
    2. Create a first connection c1 with id = 1 (in Init state)
-   3. Receive a ClientHello ch1 with random 0 on c1. Transition c1 to Sent_HRR 0 ch1
+   3. Receive a ClientHello ch1 on c1. Transition c1 to Sent_HRR 0 ch1
    4. Deallocate c1
-   5. Create a second connection c2 (in Init state)
-   6. Receive a ClientHello ch2 on c2 with a random and cookie extension matching ch1.
+   5. Create a second connection c2 with the same configuration (in Init state)
+   6. Receive a ClientHello ch2 on c2 with a cookie extension matching ch1.
    7. If the configuration of c2 is compatible with ch2,
-      a. Transition c2 to Sent_ServerHello 0 ch2 1, with c1 as the matching initial connection
-      b. Receive a ClientFinished on c2. Transition c2 to Complete 0 ch2 1
+      a. Transition c2 to Sent_ServerHello ch2 1, with c1 as the matching 
+         initial connection
+      b. Receive a ClientFinished on c2 and transition c2 to Complete ch2 1
    8. Deallocate c2
 *)
 module T = FStar.Monotonic.DependentMap
 
 let test
   (cfg:configuration)
-  (ch1:client_hello{~(has_cookie ch1) /\ ch_random ch1 == 0ul})
-  (ch2:client_hello{has_cookie ch2 /\ ch_random ch2 == 0ul})
+  (ch1:client_hello{~(has_cookie ch1)})
+  (ch2:client_hello{has_cookie ch2})
 : ST connection_table
   (requires fun _ ->
-      witnessed (region_contains_pred rgn) /\ ch_of_cookie ch2 == ch1 /\
+    witnessed (region_contains_pred rgn) /\ ch_of_cookie ch2 == ch1 /\
     ~(ch_compatible ch1 cfg))
-  (ensures  fun h0 t h1 -> 
-    if model then 
-      let t:_connection_table = t in
-      inv t h1
-    else True)
+  (ensures  fun _ t h1 -> model ==> inv t h1)
 =
-  let id1:maybe_id = if model then 1ul else () in
-  let id2:maybe_id = if model then 2ul else () in
+  let id1 = if model then 1ul else () in
+  let id2 = if model then 2ul else () in
   let t = alloc () in
   let c1 = create t id1 cfg in
   receive_client_hello1 t id1 c1 ch1;
   free_connection t id1 c1;
   let h1 = get () in
-  assert (
-    if model then
-      let t:_connection_table = t in
-      ~(T.defined t id2 h1)
-    else True);
   let c2 = create t id2 cfg in
-  if receive_client_hello2 t id2 c2 ch2 then 
-    receive_client_finished t id2 c2;
+  if receive_client_hello2 t id2 c2 ch2 then receive_client_finished t id2 c2;
   free_connection t id2 c2;
   t
